src/ecBV.ml
@@ -1,0 +1,451 @@
+(* -------------------------------------------------------------------- *)
+open EcUtils
+open EcBigInt
+open EcPath
+open EcEnv
+open EcAst
+open EcCoreFol
+open EcCoreGoal
+open EcIdent
+open LDecl
+open EcLowCircuits
+
+type ident = EcIdent.t
+
+type bvtype = 
+  [ `W of int
+  | `Int ]
+
+type op = 
+  [ `Add
+  | `Mul 
+  | `Ite
+  | `Extend of (int * bool)
+  | `Rem of bool
+  | `Div of bool
+  | `Le of bool
+  | `Lt of bool
+  | `Shls      
+  | `Shl
+  | `ASliceSet 
+  | `And
+  | `Extract   
+  | `Map
+  | `AInit     
+  | `Sub
+  | `Get       
+  | `Ror
+  | `Concat
+  | `Truncate of int
+  | `Opp
+  | `Shrs of int * bool (* Size of first operand + signed? *)
+  | `Not
+  | `Or        
+  | `Init
+  | `Insert    
+  | `Xor
+  | `Shr of bool
+  | `Mul
+  | `Rol       
+  | `A2B
+  | `ASliceGet 
+  | `B2A    
+  | `Eq ]
+
+
+let op_to_string (op: op) = 
+  match op with 
+  | `Extend (sz, true )    -> Format.sprintf "SExtend<%d>" sz
+  | `Extend (sz, false)    -> Format.sprintf "UExtend<%d>" sz
+  | `Rem true       -> "SRem"
+  | `Rem false      -> "URem"
+  | `Div true       -> "SDiv"
+  | `Div false      -> "UDiv"
+  | `Add       -> "Add"
+  | `Lt true         -> "SLt"
+  | `Lt false        -> "ULt"
+  | `Shls      -> "Shls"
+  | `Shl       -> "Shl"
+  | `ASliceSet -> "ASliceSet"
+  | `And       -> "And"
+  | `Extract   -> "Extract"
+  | `Map       -> "Map"
+  | `AInit     -> "AInit"
+  | `Sub       -> "Sub"
+  | `Get       -> "Get"
+  | `Ror       -> "Ror"
+  | `Le true        -> "SLe"
+  | `Le false       -> "ULe"
+  | `Concat    -> "Concat"
+  | `Truncate sz -> Format.sprintf "Truncate<%d>" sz
+  | `Opp       -> "Opp"
+  | `Shrs (_, true)  -> "Shras"
+  | `Shrs (_, false) -> "Shras"
+  | `Not       -> "Not"
+  | `Or        -> "Or"
+  | `Init      -> "Init"
+  | `Insert    -> "Insert"
+  | `Xor       -> "Xor"
+  | `Shr true       -> "Shra"
+  | `Shr false      -> "Shrl"
+  | `Mul       -> "Mul"
+  | `Rol       -> "Rol"
+  | `A2B       -> "A2B"
+  | `ASliceGet -> "ASliceGet"
+  | `B2A       -> "B2A"
+  | `Ite       -> "if"
+  | `Eq        -> "eq"
+
+type formula = 
+  | Base of ident * bvtype
+  | Const of int * bvtype
+  | Op of op * (formula list)
+
+let op_of_path (env: env) (p: path) : op =
+  match EcEnv.Circuit.lookup_bvoperator_path env p with
+  | Some { kind = `Extend ((_, Some bsz), (_, Some sz), sign); _} -> `Extend (sz - bsz, sign)
+  | Some { kind = `Rem ((_, Some _), sign); _}        -> `Rem sign
+  | Some { kind = `Div ((_, Some _), sign); _}        -> `Div sign
+  | Some { kind = `Add ((_, Some _)); _}        -> `Add
+  | Some { kind = `Lt ((_, Some _), sign); _}      -> `Lt sign
+  | Some { kind = `Shls _; _}       -> `Shls
+  | Some { kind = `Shl _; _}        -> `Shl
+  | Some { kind = `ASliceSet _; _}  -> `ASliceSet
+  | Some { kind = `And _; _}        -> `And
+  | Some { kind = `Extract _; _}    -> `Extract
+  | Some { kind = `Map _; _}        -> `Map
+  | Some { kind = `AInit _; _}      -> `AInit
+  | Some { kind = `Sub _; _}        -> `Sub
+  | Some { kind = `Get _; _}        -> `Get
+  | Some { kind = `Ror _; _}        -> `Ror
+  | Some { kind = `Le ((_, Some _), sign); _}     -> `Le sign
+  | Some { kind = `Concat _; _}     -> `Concat
+  | Some { kind = `Truncate ((_, Some _), (_, Some sz)); _} -> `Truncate sz
+  | Some { kind = `Opp _; _}        -> `Opp
+  | Some { kind = `Shrs ((_, Some sz), _, sign); _}       -> `Shrs (sz, sign)
+  | Some { kind = `Not _; _}        -> `Not
+  | Some { kind = `Or _; _}         -> `Or
+  | Some { kind = `Init _; _}       -> `Init
+  | Some { kind = `Insert _; _}     -> `Insert
+  | Some { kind = `Xor _; _}        -> `Xor
+  | Some { kind = `Shr ((_, Some _), sign); _}  -> `Shr sign
+  | Some { kind = `Mul _; _}        -> `Mul
+  | Some { kind = `Rol _; _}        -> `Rol
+  | Some { kind = `A2B _; _}        -> `A2B
+  | Some { kind = `ASliceGet _; _}  -> `ASliceGet
+  | Some { kind = `B2A _; _}        -> `B2A
+  | _ -> Format.eprintf "Failed for path %s@." (EcPath.tostring p);
+    assert false
+
+let bvtype_of_ty env ty : bvtype = 
+  if ty = EcTypes.tint then
+    `Int
+  else `W (size_of_ctype @@ EcCircuits.ctype_of_ty env ty)
+
+let pp_bvtype fmt t : unit =
+  match t with
+  | `W i -> Format.fprintf fmt "@%d" i
+  | `Int -> Format.fprintf fmt "Z"
+
+let rec pp_formula fmt f : unit =
+  match f with
+  | Base (id, t) -> Format.fprintf fmt "%s[%a]" id.id_symb pp_bvtype t
+  | Op (op, args) -> Format.fprintf fmt "%s(@[<hov 2>%a@])" (op_to_string op) 
+    EcPrinting.(pp_list "," pp_formula) args
+  | Const (i, t) -> Format.fprintf fmt "%d[%a]" i pp_bvtype t
+
+let bvformula_of_form (hyps: hyps) (f: form) : formula = 
+  let env = toenv hyps in
+
+  let pv_cache : (prog_var * ident, ident) Map.t ref = ref Map.empty in
+  let let_binds : (ident, formula) Map.t = Map.empty in
+
+  let rec doit lbinds (f_: form) =
+    match f_.f_node with
+    | Fquant (_, _, _) -> assert false
+    | Fif (c, t, f) -> 
+      let c = doit lbinds c in
+      let t = doit lbinds t in
+      let f = doit lbinds f in
+      Op (`Ite, [c; t; f])
+    | Fmatch (_, _, _) -> assert false
+    | Flet (lp, v, e) -> begin 
+      match lp with
+      | LSymbol (id, _t) -> 
+        let v_bv = doit lbinds v in
+        let lbinds = Map.add id v_bv lbinds in
+        doit lbinds e
+      | _ -> assert false
+      end
+    | Fint z -> Const (BI.to_int z, `Int)
+    | Flocal lv -> begin match Map.find_opt lv lbinds with
+      | Some f -> f
+      | None -> Base (lv, bvtype_of_ty env f_.f_ty)
+      end
+    | Fpvar (pv, m) -> 
+      let id = match Map.find_opt (pv, m) !pv_cache with
+      | Some id -> id
+      | None -> let name = match pv with
+        | PVglob _ -> assert false
+        | PVloc s -> s
+        in let id = EcIdent.create name in
+        pv_cache := Map.add (pv, m) id !pv_cache;
+        id
+      in
+      Base (id, bvtype_of_ty env f_.f_ty)
+    | Fglob (_, _) -> assert false
+    | Fop (_, _) -> assert false
+    | Fapp ({f_node = Fop(p, _);}, [arg]) when (EcPath.toqsymbol p |> snd) = "of_int" ->
+      Const (EcCircuits.int_of_form hyps arg |> BI.to_int, 
+             `W (EcEnv.Circuit.lookup_bitstring_size env f_.f_ty |> Option.get))
+    | Fapp (_, _) -> 
+        let (fp, _), fs = destr_op_app f_ in
+        let args = List.map (doit lbinds) fs in
+        begin match EcFol.op_kind fp with
+        | Some `Eq ->
+          Op (`Eq, args)
+        | _ -> 
+          let op = op_of_path env fp in
+          Op (op, args)
+        end
+    | Ftuple _ -> assert false
+
+    | Fproj (_, _) -> assert false
+
+    | FhoareF _ -> assert false
+    | FhoareS _ -> assert false
+    | FbdHoareF _ -> assert false
+    | FbdHoareS _ -> assert false
+    | FeHoareF _ -> assert false
+    | FeHoareS _ -> assert false
+    | FequivF _ -> assert false
+    | FequivS _ -> assert false
+    | FeagerF _ -> assert false
+    | Fpr _ -> assert false
+  in 
+  doit let_binds f
+
+
+let check_formula_BWZ (f: formula) : bool = 
+  let open Bitwuzla_cxx in
+  let options = Options.default () in
+  Options.set options Produce_models true;
+  let bitwuzla = Solver.create options in
+
+
+  let bvterm_of_int (size: int) (v: int) : Term.t =
+    mk_bv_value_int (mk_bv_sort size) v
+  in
+
+  let bvterm_of_ident (size: int) (id: ident) : Term.t = 
+    mk_const (mk_bv_sort size) ~symbol:(id.id_symb ^ "#" ^ (string_of_int id.id_tag))
+  in
+
+  let size_of_bvtype ty = 
+    match ty with 
+    | `W s -> s
+    | _ -> assert false
+  in
+
+  let base_terms : (ident, Term.t) Map.t ref = ref Map.empty in
+
+  let rec doit (f: formula) : Term.t = 
+    match f with
+    | Base (id, t) -> 
+      begin match Map.find_opt id !base_terms with
+      | Some t -> t
+      | None -> let t = bvterm_of_ident (size_of_bvtype t) id in
+        base_terms := Map.add id t !base_terms;
+        t
+      end
+    | Const (v, t) -> bvterm_of_int (size_of_bvtype t) v
+    | Op (op, args) ->
+      let args = List.map doit args in
+      begin try begin match op, args with
+      | `Extend (sz, true),  [bv] -> mk_term1_indexed1 Kind.Bv_sign_extend bv sz
+      | `Extend (sz, false), [bv] -> mk_term1_indexed1 Kind.Bv_zero_extend bv sz
+      | `Rem true,  [bv1; bv2] -> mk_term2 Kind.Bv_srem bv1 bv2
+      | `Rem false, [bv1; bv2] -> mk_term2 Kind.Bv_urem bv1 bv2
+      | `Div true , [bv1; bv2] -> mk_term2 Kind.Bv_sdiv bv1 bv2
+      | `Div false, [bv1; bv2] -> mk_term2 Kind.Bv_udiv bv1 bv2 
+      | `Add, [bv1; bv2] -> mk_term2 Kind.Bv_add bv1 bv2
+      | `Shl, [bv1; bv2] -> mk_term2 Kind.Bv_shl bv1 bv2
+      | `Shls, args -> assert false
+      | `Lt true,  [bv1; bv2] -> mk_term2 Kind.Bv_slt bv1 bv2
+      | `Lt false, [bv1; bv2] -> mk_term2 Kind.Bv_ult bv1 bv2
+      | `ASliceSet, args -> assert false
+      | `And, [bv1; bv2] -> mk_term2 Kind.Bv_and bv1 bv2
+      | `Extract, args -> assert false
+      | `Map, args -> assert false
+      | `Ite, [c; t; f] -> assert false
+      | `AInit, args -> assert false
+      | `Sub, [bv1; bv2] -> mk_term2 Kind.Bv_sub bv1 bv2
+      | `Ror, [bv1; bv2] -> mk_term2 Kind.Bv_ror bv1 bv2
+      | `Get, args -> assert false
+      | `Le true , [bv1; bv2] -> mk_term2 Kind.Bv_sle bv1 bv2
+      | `Le false, [bv1; bv2] -> mk_term2 Kind.Bv_ule bv1 bv2
+      | `Opp, [bv] -> mk_term1 Kind.Bv_neg bv
+      | `Truncate sz, [bv] -> mk_term1_indexed2 Kind.Bv_extract bv (sz-1) 0
+      | `Concat, [bv1; bv2] -> mk_term2 Kind.Bv_concat bv1 bv2
+      | `Shrs (sz, true ), [bv1; bv2] -> 
+        mk_term2 Kind.Bv_ashr bv1 (mk_term1_indexed1 Kind.Bv_zero_extend bv2 (sz - 8))
+      | `Shrs (sz, false), [bv1; bv2] -> 
+        mk_term2 Kind.Bv_shr bv1 (mk_term1_indexed1 Kind.Bv_zero_extend bv2 (sz - 8))
+      | `Or, [bv1; bv2] -> mk_term2 Kind.Bv_or bv1 bv2
+      | `Not, [bv] -> mk_term1 Kind.Bv_not bv
+      | `Shr true , [bv1; bv2] -> mk_term2 Kind.Bv_ashr bv1 bv2
+      | `Shr false, [bv1; bv2] -> mk_term2 Kind.Bv_shr bv1 bv2
+      | `Xor, [bv1; bv2] -> mk_term2 Kind.Bv_xor bv1 bv2
+      | `Insert, args -> assert false
+      | `Init, args -> assert false
+      | `Mul, [bv1; bv2] -> mk_term2 Kind.Bv_mul bv1 bv2
+      | `Rol, [bv1; bv2] -> mk_term2 Kind.Bv_rol bv1 bv2
+      | `A2B, args -> assert false
+      | `ASliceGet, args -> assert false
+      | `B2A, args -> assert false
+      | `Eq, [bv1; bv2] -> mk_term2 Kind.Equal bv1 bv2
+      | _ -> assert false
+      end
+    with e ->
+      Format.eprintf "Failed on formula %a@." pp_formula f;
+      raise e
+    end
+  in 
+  Solver.assert_formula bitwuzla (mk_term1 Kind.Not @@ doit f);
+
+  let get_val (bv: Term.t) : Term.t =
+    Solver.get_value bitwuzla bv 
+  in
+  match Solver.check_sat bitwuzla with
+  | Sat -> 
+    Map.iter (fun _ t ->
+      Format.eprintf "%a: %a@." Term.pp t Term.pp (get_val t)) !base_terms;
+    false
+  | Unsat -> true
+  | Unknown -> assert false
+  
+let check_equality_BWZ (f1: formula) (f2: formula) : bool = 
+  let open Bitwuzla_cxx in
+  let options = Options.default () in
+  Options.set options Produce_models true;
+  let bitwuzla = Solver.create options in
+
+
+  let bvterm_of_int (size: int) (v: int) : Term.t =
+    mk_bv_value_int (mk_bv_sort size) v
+  in
+
+  let bvterm_of_ident (size: int) (id: ident) : Term.t = 
+    mk_const (mk_bv_sort size) ~symbol:(id.id_symb ^ "#" ^ (string_of_int id.id_tag))
+  in
+
+  let size_of_bvtype ty = 
+    match ty with 
+    | `W s -> s
+    | _ -> assert false
+  in
+
+  let base_terms : (ident, Term.t) Map.t ref = ref Map.empty in
+
+  let rec doit (f: formula) : Term.t = 
+    match f with
+    | Base (id, t) -> 
+      begin match Map.find_opt id !base_terms with
+      | Some t -> t
+      | None -> let t = bvterm_of_ident (size_of_bvtype t) id in
+        base_terms := Map.add id t !base_terms;
+        t
+      end
+    | Const (v, t) -> bvterm_of_int (size_of_bvtype t) v
+    | Op (op, args) ->
+      let args = List.map doit args in
+      begin try begin match op, args with
+      | `Extend (sz, true),  [bv] -> mk_term1_indexed1 Kind.Bv_sign_extend bv sz
+      | `Extend (sz, false), [bv] -> mk_term1_indexed1 Kind.Bv_zero_extend bv sz
+      | `Rem true,  [bv1; bv2] -> mk_term2 Kind.Bv_srem bv1 bv2
+      | `Rem false, [bv1; bv2] -> mk_term2 Kind.Bv_urem bv1 bv2
+      | `Div true , [bv1; bv2] -> mk_term2 Kind.Bv_sdiv bv1 bv2
+      | `Div false, [bv1; bv2] -> mk_term2 Kind.Bv_udiv bv1 bv2 
+      | `Add, [bv1; bv2] -> mk_term2 Kind.Bv_add bv1 bv2
+      | `Shl, [bv1; bv2] -> mk_term2 Kind.Bv_shl bv1 bv2
+      | `Shls, args -> assert false
+      | `Lt true,  [bv1; bv2] -> mk_term2 Kind.Bv_slt bv1 bv2
+      | `Lt false, [bv1; bv2] -> mk_term2 Kind.Bv_ult bv1 bv2
+      | `ASliceSet, args -> assert false
+      | `And, [bv1; bv2] -> mk_term2 Kind.Bv_and bv1 bv2
+      | `Extract, args -> assert false
+      | `Map, args -> assert false
+      | `Ite, [c; t; f] -> assert false
+      | `AInit, args -> assert false
+      | `Sub, [bv1; bv2] -> mk_term2 Kind.Bv_sub bv1 bv2
+      | `Ror, [bv1; bv2] -> mk_term2 Kind.Bv_ror bv1 bv2
+      | `Get, args -> assert false
+      | `Le true , [bv1; bv2] -> mk_term2 Kind.Bv_sle bv1 bv2
+      | `Le false, [bv1; bv2] -> mk_term2 Kind.Bv_ule bv1 bv2
+      | `Opp, [bv] -> mk_term1 Kind.Bv_neg bv
+      | `Truncate sz, [bv] -> mk_term1_indexed2 Kind.Bv_extract bv (sz-1) 0
+      | `Concat, [bv1; bv2] -> mk_term2 Kind.Bv_concat bv1 bv2
+      | `Shrs (sz, true ), [bv1; bv2] -> 
+        mk_term2 Kind.Bv_ashr bv1 (mk_term1_indexed1 Kind.Bv_zero_extend bv2 (sz - 8))
+      | `Shrs (sz, false), [bv1; bv2] -> 
+        mk_term2 Kind.Bv_shr bv1 (mk_term1_indexed1 Kind.Bv_zero_extend bv2 (sz - 8))
+      | `Or, [bv1; bv2] -> mk_term2 Kind.Bv_or bv1 bv2
+      | `Not, [bv] -> mk_term1 Kind.Bv_not bv
+      | `Shr true , [bv1; bv2] -> mk_term2 Kind.Bv_ashr bv1 bv2
+      | `Shr false, [bv1; bv2] -> mk_term2 Kind.Bv_shr bv1 bv2
+      | `Xor, [bv1; bv2] -> mk_term2 Kind.Bv_xor bv1 bv2
+      | `Insert, args -> assert false
+      | `Init, args -> assert false
+      | `Mul, [bv1; bv2] -> mk_term2 Kind.Bv_mul bv1 bv2
+      | `Rol, [bv1; bv2] -> mk_term2 Kind.Bv_rol bv1 bv2
+      | `A2B, args -> assert false
+      | `ASliceGet, args -> assert false
+      | `B2A, args -> assert false
+      | `Eq, [bv1; bv2] -> mk_term2 Kind.Equal bv1 bv2
+      | _ -> assert false
+      end
+    with e ->
+      Format.eprintf "Failed on formula %a@." pp_formula f;
+      raise e
+    end
+  in 
+  let bv1 = doit f1 in
+  let bv2 = doit f2 in
+  Solver.assert_formula bitwuzla (mk_term2 Kind.Distinct bv1 bv2);
+  let get_val (bv: Term.t) : Term.t =
+    Solver.get_value bitwuzla bv
+  in
+  match Solver.check_sat bitwuzla with
+  | Sat -> 
+    Map.iter (fun _ t ->
+      Format.eprintf "%a: %a@." Term.pp t Term.pp (get_val t)) !base_terms;
+    false
+  | Unsat -> true
+  | Unknown -> assert false
+
+let t_solve (tc: tcenv1) : tcenv =
+  match (FApi.tc1_goal tc) with
+  | f when f.f_ty = EcTypes.tbool -> 
+    begin match EcFol.sform_of_form f with
+(*
+    | EcFol.SFeq (f1, f2) ->
+      Format.eprintf "Checking equality@.";
+      let bv1 = bvformula_of_form (FApi.tc1_hyps tc) f1 in
+      let bv2 = bvformula_of_form (FApi.tc1_hyps tc) f2 in
+      if check_equality_BWZ bv1 bv2 then
+        Format.eprintf "Success@."
+      else 
+        Format.eprintf "Fail@.";
+      assert false
+*)
+    | _ ->
+      let f = bvformula_of_form (FApi.tc1_hyps tc) f in
+      Format.eprintf "%a@." pp_formula f;
+      if check_formula_BWZ f then
+        Format.eprintf "Success@."
+      else 
+        Format.eprintf "Fail@.";
+      assert false
+    end
+  | _ -> assert false
+
